speed up NewBaseystem synthesis
Use a vm_compute hack fromhttps://arxiv.org/pdf/1305.6543.pdf section 5.5:
pattern terms over what to keep opaque, then reduce the lambda using
vm_compute.

src/NewBaseSystem.v
@@ -1,15 +1,3 @@
-Require Import Coq.ZArith.ZArith Coq.micromega.Psatz Coq.omega.Omega.
-Require Import Coq.ZArith.BinIntDef.
-Local Open Scope Z_scope.
-
-Require Import Crypto.Tactics.Algebra_syntax.Nsatz.
-Require Import Crypto.Util.Tactics Crypto.Util.Decidable Crypto.Util.LetIn.
-Require Import Crypto.Util.ZUtil Crypto.Util.ListUtil Crypto.Util.Sigma.
-Require Import Crypto.Util.CPSUtil Crypto.Util.Prod.
-
-Require Import Coq.Lists.List. Import ListNotations.
-Require Crypto.Util.Tuple. Local Notation tuple := Tuple.tuple.
-
 (*****
 
 This file provides a generalized version of arithmetic with "mixed
@@ -252,6 +240,17 @@ reasonable time, so this is not really an option.
 
 *****)
 
+Require Import Coq.ZArith.ZArith Coq.micromega.Psatz Coq.omega.Omega.
+Require Import Coq.ZArith.BinIntDef.
+Local Open Scope Z_scope.
+
+Require Import Crypto.Tactics.Algebra_syntax.Nsatz.
+Require Import Crypto.Util.Tactics Crypto.Util.Decidable Crypto.Util.LetIn.
+Require Import Crypto.Util.ZUtil Crypto.Util.ListUtil Crypto.Util.Sigma.
+Require Import Crypto.Util.CPSUtil Crypto.Util.Prod Crypto.Util.Tactics.
+
+Require Import Coq.Lists.List. Import ListNotations.
+Require Crypto.Util.Tuple. Local Notation tuple := Tuple.tuple.
 
 Local Ltac prove_id :=
   repeat match goal with
@@ -640,6 +639,10 @@ Module B.
       Proof. cbv [carry_cps carry]; intros; eapply @eval_carry; eauto. Qed.
       Hint Rewrite @eval_carry : push_basesystem_eval.
 
+      (* TODO make a correctness proof for this *)
+      Definition chained_carries (p:list limb) (idxs : list nat)
+                 {T} (f:list limb->T) :=
+        fold_right_cps2 carry_cps p idxs f.
       End Carries.
     End Positional.
   End Positional.
@@ -675,6 +678,27 @@ Local Coercion Z.of_nat : nat >-> Z.
 Import Coq.Lists.List.ListNotations. Local Open Scope list_scope.
 Import B.
 
+Ltac basesystem_partial_evaluation_RHS := 
+  let t0 := match goal with |- _ _ ?t => t end in
+  let t := (eval cbv delta [
+  (* this list must contain all definitions referenced by t that reference [Let_In], [runtime_add], or [runtime_mul] *)
+Positional.to_associational_cps Positional.to_associational Positional.eval Positional.zeros Positional.add_to_nth_cps Positional.add_to_nth Positional.place_cps Positional.place Positional.from_associational_cps Positional.from_associational Positional.carry_cps Positional.carry Positional.chained_carries
+Associational.eval Associational.multerm Associational.mul_cps Associational.mul Associational.split_cps Associational.split Associational.reduce_cps Associational.reduce Associational.carryterm_cps Associational.carryterm Associational.carry_cps Associational.carry Associational.sat_multerm_cps Associational.sat_multerm Associational.sat_mul_cps Associational.sat_mul
+                 ] in t0) in
+  let t := (eval pattern @runtime_mul in t) in
+  let t := match t with ?t _ => t end in
+  let t := (eval pattern @runtime_add in t) in
+  let t := match t with ?t _ => t end in
+  let t := (eval pattern @Let_In in t) in
+  let t := match t with ?t _ => t end in
+  let t1 := fresh "t1" in
+  pose t as t1;
+  transitivity (t1
+                  (@Let_In)
+                  (@runtime_add)
+                  (@runtime_mul));
+  [replace_with_vm_compute t1; clear t1|reflexivity].
+
 Ltac assert_preconditions :=
   repeat match goal with
          | |- context [Positional.from_associational_cps ?wt ?n] =>
@@ -686,24 +710,6 @@ Ltac assert_preconditions :=
          | |- context [Positional.carry_cps?wt ?i] =>
            unique assert (wt (S i) / wt i <> 0) by (cbv; congruence)
          end.
-
-Ltac op_simplify := 
-  cbv - [runtime_add runtime_mul Let_In];
-  cbv [runtime_add runtime_mul].
-
-Ltac prove_op sz x :=
-  cbv [Tuple.tuple Tuple.tuple'] in *;
-  repeat match goal with p : _ * Z |- _ => destruct p end;
-  apply lift2_sig;
-  eexists; cbv zeta beta; intros;
-  match goal with |- Positional.eval ?wt _ = ?op (Positional.eval ?wt ?a) (Positional.eval ?wt ?b) =>
-                  transitivity (Positional.eval wt (x wt a b))
-  end; 
-  [ apply f_equal; op_simplify; reflexivity
-  | assert_preconditions;
-    progress autorewrite with uncps push_id push_basesystem_eval;
-    reflexivity ]
-.
 
 Section Ops.
   Context
@@ -717,23 +723,26 @@ Section Ops.
   Let sz := 10%nat.
   Let sz2 := Eval compute in ((sz * 2) - 1)%nat.
 
-  (* shorthand for many carries in a row *)
-  Definition chained_carries (w : nat -> Z) (p:list B.limb) (idxs : list nat)
-             {T} (f:list B.limb->T) :=
-    fold_right_cps2 (@Positional.carry_cps w modulo div) p idxs f.
-
   Definition addT :
     { add : (Z^sz -> Z^sz -> Z^sz)%type &
                forall a b : Z^sz,
                  let eval {n} := Positional.eval (n := n) wt in
                  eval (add a b) = eval a  + eval b }.
   Proof.
-    prove_op sz (
-        fun wt a b =>
+    let x := constr:(fun wt a b =>
         Positional.to_associational_cps (n := sz) wt a
           (fun r => Positional.to_associational_cps (n := sz) wt b
           (fun r0 => Positional.from_associational_cps wt sz (r ++ r0) id
-        ))).
+        ))) in
+    apply lift2_sig; eexists;
+    transitivity (Positional.eval wt (x wt a b));
+      [|assert_preconditions; autorewrite with uncps push_id push_basesystem_eval; reflexivity].
+
+    apply f_equal.
+    
+    basesystem_partial_evaluation_RHS.
+
+    reflexivity.
   Defined.
   
 
@@ -743,19 +752,31 @@ Section Ops.
                  let eval {n} := Positional.eval (n := n) wt in
                  eval (mul a b) = eval a  * eval b }.
   Proof.
-    let x := (eval cbv [chained_carries seq fold_right_cps2 sz2] in
-        (fun w a b =>
+    let x := constr:(fun w a b =>
          Positional.to_associational_cps (n := sz) w a
            (fun r => Positional.to_associational_cps (n := sz) w b
            (fun r0 => Associational.mul_cps r r0
            (fun r1 => Positional.from_associational_cps w sz2 r1
            (fun r2 => Positional.to_associational_cps w r2
-           (fun r3 => chained_carries w r3 (seq 0 sz2)
+           (fun r3 => Positional.chained_carries(div:=div)(modulo:=modulo) w r3 (seq 0 sz2)
            (fun r13 => Positional.from_associational_cps w sz2 r13 id
-             )))))))) in
-    prove_op sz x.
-  Defined.
+             ))))))) in
+    apply lift2_sig; eexists;
+    transitivity (Positional.eval wt (x wt a b));
+      [|cbv [Positional.chained_carries fold_right_cps2 seq fold_right sz2]; assert_preconditions; autorewrite with uncps push_id push_basesystem_eval; reflexivity].
 
+    apply f_equal.
+
+    basesystem_partial_evaluation_RHS.
+
+    (* rough breakdown of synthesis time *)
+    (* 1.2s for side conditions -- should improve significantly when [chained_carries] gets a correctness lemma *)
+    (* basesystem_partial_evaluation_RHS (primarily vm_compute): 1.8s, which gets re-computed during defined *)
+
+    (* doing [cbv -[Let_In runtime_add runtime_mul]] took 37s *)
+
+    reflexivity.
+  Defined. (* 3s *)
 End Ops.
 
 (*
