src/Util/Tactics/VM.v
@@ -1,0 +1,32 @@
+(* Code by Jason Gross for COQBUG 4637: vm_compute in _ makes Defined slow *)
+
+(** First, work around COQBUG 4494, https://coq.inria.fr/bugs/show_bug.cgi?id=4494 (replace is slow and broken under binders *)
+Ltac replace_with_at_by x y set_tac tac :=
+  let H := fresh in
+  let x' := fresh in
+  set_tac x' x;
+  assert (H : y = x') by (subst x'; tac);
+  clearbody x'; induction H.
+
+Ltac replace_with_at x y set_tac :=
+  let H := fresh in
+  let x' := fresh in
+  set_tac x' x;
+  cut (y = x');
+  [ intro H; induction H
+  | subst x' ].
+
+Ltac replace_with_vm_compute c :=
+  let c' := (eval vm_compute in c) in
+  (* we'd like to just do: *)
+  (* replace c with c' by (clear; abstract (vm_compute; reflexivity)) *)
+  (* but [set] is too slow in 8.4, so we write our own version (see COQBUG https://coq.inria.fr/bugs/show_bug.cgi?id=3280#c13 *)
+  let set_tac := (fun x' x
+                  => pose x as x';
+                     change x with x') in
+  replace_with_at_by c c' set_tac ltac:(clear; vm_cast_no_check (eq_refl c')).
+
+Ltac replace_with_vm_compute_in c H :=
+  let c' := (eval vm_compute in c) in
+  (* By constrast [set ... in ...] seems faster than [change .. with ... in ...] in 8.4?! *)
+  replace_with_at_by c c' ltac:(fun x' x => set (x' := x) in H ) ltac:(clear; vm_cast_no_check (eq_refl c')).
